high2/Zeta.High.Interleave.fst
@@ -1,8 +1,36 @@
 module Zeta.High.Interleave
 
-let mk_vlog_entry_ext (#app: app_params) (#n:nat)
-  : IF.idxfn_t (gen_seq app n) (vlog_entry_ext app)
-  = admit()
+let mk_vlog_entry_ext #app #n (il: verifiable_log app n) (i: seq_index il)
+  = let vle = I.index il i in
+    let open Zeta.GenericVerifier in
+    let open Zeta.High.Verifier in
+    let vs = cur_thread_state_pre il i in
+    lemma_cur_thread_state_extend il i;
+
+    match vle with
+    | EvictM k k' ->
+      let v = stored_value vs.st k in
+      EvictMerkle vle v
+    | EvictB k ts ->
+      let v = stored_value vs.st k in
+      let tid = vs.tid in
+      EvictBlum vle v tid
+    | EvictBM k _ ts ->
+      let v = stored_value vs.st k in
+      let tid = vs.tid in
+      EvictBlum vle v tid
+    | RunApp f p ss ->
+      assert(Some? (get_record_set ss vs));
+      assert(SA.distinct_elems ss);
+      let rs = get_record_set_succ ss vs in
+      App vle rs
+    | v -> NEvict v
+
+let vlog_entry_ext_prop (#app #n:_) (il: verifiable_log app n) (i: seq_index il)
+  : Lemma (ensures (let ee = mk_vlog_entry_ext il i in
+                    let e = I.index il i in
+                    e = to_vlog_entry ee))
+  = ()
 
 let is_eac_post (#app: app_params) (#n:nat)
   (il: verifiable_log app n) (i: seq_index il)
@@ -19,16 +47,6 @@ let lemma_eac_empty #app #n (il: verifiable_log app n{S.length il = 0})
   = let le = vlog_ext_of_il_log il in
     eac_empty_log le
 
-let eac_boundary (#app #n:_) (il: neac_log app n)
-  : (i: seq_index il{is_eac (prefix il i) /\
-                     ~ (is_eac (prefix il (i+1)))})
-  = let open Zeta.IdxFn in
-    let le = vlog_ext_of_il_log il in
-    let i = max_eac_prefix le in
-    lemma_map_prefix mk_vlog_entry_ext il i;
-    lemma_map_prefix mk_vlog_entry_ext il (i+1);
-    i
-
 let lemma_eac_implies_prefix_eac (#app #n:_) (il: verifiable_log app n) (i: nat{i <= S.length il})
   : Lemma (ensures (is_eac il ==> is_eac (prefix il i)))
   = let open Zeta.IdxFn in
@@ -40,3 +58,34 @@ let lemma_eac_implies_appfn_calls_seq_consistent (#app #n:_) (il: eac_log app n)
   : Lemma (ensures (let gl = to_glog il in
                     Zeta.AppSimulate.seq_consistent (G.appfn_calls gl)))
   = admit()
+
+let eac_boundary (#app #n:_) (il: neac_log app n)
+  : (i: seq_index il{is_eac (prefix il i) /\
+                     ~ (is_eac (prefix il (i+1)))})
+  = let open Zeta.IdxFn in
+    let le = vlog_ext_of_il_log il in
+    let i = max_eac_prefix le in
+    lemma_map_prefix mk_vlog_entry_ext il i;
+    lemma_map_prefix mk_vlog_entry_ext il (i+1);
+    i
+
+let eac_boundary_not_appfn (#app #n:_) (il: neac_log app n)
+  : Lemma (ensures (let i = eac_boundary il in
+                    let e = I.index il i in
+                    not (V.is_appfn e)))
+  = let i = eac_boundary il in
+    let e = I.index il i in
+    let ee = mk_vlog_entry_ext il i in
+    let le = vlog_ext_of_il_log il in
+    let k = eac_fail_key le in
+    let smk = eac_smk app k in
+    let lei = SA.prefix le i in
+    let lei' = SA.prefix le (i+1) in
+    let open Zeta.SeqMachine in
+    assert(valid smk lei);
+    assert(~ (valid smk lei'));
+
+    if V.is_appfn e then (
+      admit()
+    )
+    else ()
